\chapter{Choice of ACE Variables}
\label{app:ace}

\begin{remark}
    Recall the affine approach to steering from \cref{eq:ace}
    \begin{equation*}
        \va_\text{\normalfont steered} = \va - \text{\normalfont proj}_\vr^{\parallel}(\va) + \alpha_0\vr + \alpha\vr.
    \end{equation*}
    Given a set of positive example activations $\{\va_i^+\}_i$ and negative example activations $\{\va_i^-\}_i$ the appropriate choices for $\alpha_0$ and $\vr$ are
    \begin{equation}
        \label{eq:ace-app}
        \begin{aligned}
            \vr = \frac{1}{n}\sum_{i=1}^{n}\left(\va_i^+ - \va_i^-\right) && \alpha_0 = \text{\normalfont proj}_\vr^\parallel\left(\frac{1}{n}\sum_{i=1}^{n}\va_i^-\right)
        \end{aligned}
    \end{equation}
\end{remark}
\begin{proof}
    Let $\mu_{\va^+} = \frac{1}{n}\sum_{i=1}^{n}\va_i^+$ be the mean of the positive activations and $\mu_{\va^-}$ the mean of the negative activation.
    It is safe to assume that $\vr \in \text{span}(\mu_{\va^+} - \mu_{\va^-})$

    When $\alpha = 0$ the expected behaviour of the model should be neutral and when $\alpha = 1$ the expected behaviour should be the target behaviour.
    Therefore
    \begin{equation*}
        \begin{aligned}
            \mathbb{E}_{\alpha=0}[\va_\text{steered}] &= \mathbb{E}_\text{neutral-behaviour}[\va] = \mu_{\va^-} \\
            \mathbb{E}_{\alpha=1}[\va_\text{steered}] &= \mathbb{E}_\text{target-behaviour}[\va] = \mu_{\va^+}.
        \end{aligned}
    \end{equation*}

    Considering the first equation note that
    \begin{equation*}
        \begin{aligned}
            \mathbb{E}_{\alpha=0}[\va - \text{proj}_\vr^{\parallel}(\va) + \alpha_0\vr + \alpha\vr] &=  \mathbb{E}[\va - \text{proj}_\vr^{\parallel}(\va) + \alpha_0\vr] = \mu_{\va^-}.
        \end{aligned}
    \end{equation*}
    Taking the projection parallel to $\vr$ to both sides provides a definition for $\alpha_0$
    \begin{equation*}
        \begin{aligned}
            \text{proj}_\vr^{\parallel}(\mathbb{E}[\va - \text{proj}_\vr^{\parallel}(\va) + \alpha_0\vr]) &= \text{proj}_\vr^{\parallel}(\mu_{\va^-}) \\
            \implies \mathbb{E}[\text{proj}_\vr^{\parallel}(\va) - \text{proj}_\vr^{\parallel}(\va) + \alpha_0\text{proj}_\vr^{\parallel}(\vr)] &= \text{proj}_\vr^{\parallel}(\mu_{\va^-}) \\
            \implies \alpha_0\vr &= \text{proj}_\vr^{\parallel}(\mu_{\va^-}).
        \end{aligned}
    \end{equation*}

    Considering the second equation provides a similar result
    \begin{equation*}
        \text{proj}_\vr^{\parallel}(\mathbb{E}[\va - \text{proj}_\vr^{\parallel}(\va) + \alpha_0\vr + \vr]) = \alpha_0\vr + \vr = \text{proj}_\vr^{\parallel}(\mu_{\va^+}).
    \end{equation*}

    Subtracting these results provides a definition for $\vr$
    \begin{equation*}
        \vr = \text{proj}_\vr^{\parallel}(\mu_{\va^+}) - \text{proj}_\vr^{\parallel}(\mu_{\va^-}) = \text{proj}_\vr^{\parallel}(\mu_{\va^+} - \mu_{\va^-}).
    \end{equation*}
    As $\vr \in \text{span}(\mu_{\va^+} - \mu_{\va^-})$ the tighter bound
    \begin{equation*}
        \vr = \mu_{\va^+} - \mu_{\va^-} = \frac{1}{n}\sum_{i=1}^{n}\va_i^+ - \frac{1}{n}\sum_{i=1}^{n}\va_i^- = \frac{1}{n}\sum_{i=1}^{n}(\va_i^+ - \va_i^-)
    \end{equation*}
    is found.
    This leads to the result for $\alpha_0$ and $\vr$ in \cref{eq:ace-app}.
\end{proof}
